Restore hashtable

pulse/share/steel/examples/pulse/lib/Pulse.Lib.HashTable.fst
@@ -10,702 +10,693 @@ open Pulse.Lib.HashTable.Type
 
 #push-options "--using_facts_from '* -FStar.Tactics -FStar.Reflection'"
 
-// let mk_used_cell (#a:eqtype) #b (k:a) (v:b) : cell a b = Used k v
+let mk_used_cell (#a:eqtype) #b (k:a) (v:b) : cell a b = Used k v
 
-// let mk_ht (#k:eqtype) #v 
-//           (sz:pos_us) 
-//           (hashf:k -> SZ.t)
-//           (contents:V.vec (cell k v))
-//   : ht_t k v
-//   = { sz; hashf; contents; }
+let mk_ht (#k:eqtype) #v 
+          (sz:pos_us) 
+          (hashf:k -> SZ.t)
+          (contents:V.vec (cell k v))
+  : ht_t k v
+  = { sz; hashf; contents; }
 
-// let lift_hash_fun (#k:eqtype) (hashf:k -> SZ.t) : GTot (k -> nat) = fun k -> SZ.v (hashf k)
+let lift_hash_fun (#k:eqtype) (hashf:k -> SZ.t) : GTot (k -> nat) = fun k -> SZ.v (hashf k)
 
-// let mk_init_pht (#k:eqtype) #v (hashf:k -> SZ.t) (sz:pos_us)
-//   : GTot (pht_t k v)
-//   = 
-//   { spec = (fun k -> None);
-//     repr = {
-//       sz=SZ.v sz;
-//       seq=Seq.create (SZ.v sz) Clean;
-//       hashf=lift_hash_fun hashf;
-//     };
-//     inv = (); }
+let mk_init_pht (#k:eqtype) #v (hashf:k -> SZ.t) (sz:pos_us)
+  : GTot (pht_t k v)
+  = 
+  { spec = (fun k -> None);
+    repr = {
+      sz=SZ.v sz;
+      seq=Seq.create (SZ.v sz) Clean;
+      hashf=lift_hash_fun hashf;
+    };
+    inv = (); }
 
-// noextract
-// let related #kt #vt (ht:ht_t kt vt) (pht:pht_t kt vt) : GTot prop =
-//   SZ.v ht.sz == pht.repr.sz /\
-//   pht.repr.hashf == lift_hash_fun ht.hashf
+noextract
+let related #kt #vt (ht:ht_t kt vt) (pht:pht_t kt vt) : GTot prop =
+  SZ.v ht.sz == pht.repr.sz /\
+  pht.repr.hashf == lift_hash_fun ht.hashf
 
 let models #kt #vt (ht:ht_t kt vt) (pht:pht_t kt vt) : vprop =
   V.pts_to ht.contents pht.repr.seq
-  // **
-  // pure ( related ht pht /\ V.is_full_vec ht.contents)
+  **
+  pure ( related ht pht /\ V.is_full_vec ht.contents)
 
-// let pht_sz #k #v (pht:pht_t k v) : GTot pos = pht.repr.sz
+let pht_sz #k #v (pht:pht_t k v) : GTot pos = pht.repr.sz
 
 ```pulse
-fn tmp (#k:eqtype) (#v:Type0) (ht:ht_t k v) (pht:erased (pht_t k v))
-  requires V.pts_to ht.contents pht.repr.seq
-  ensures models ht pht
+fn alloc (#k:eqtype) (#v:Type0) (hashf:(k -> SZ.t)) (l:pos_us)
+  requires emp
+  returns ht:ht_t k v
+  ensures exists* pht. models ht pht ** pure (pht == mk_init_pht hashf l)
 {
-  fold models
+  let contents = V.alloc #(cell k v) Clean l;
+  let ht = mk_ht l hashf contents;
+  let pht = Ghost.hide (mk_init_pht #k #v hashf l);
+  rewrite (V.pts_to contents (Seq.create (SZ.v l) Clean))
+       as (V.pts_to ht.contents pht.repr.seq);
+  fold models;
+  admit ()
 }
 ```
 
-// ```pulse
-// fn alloc (#k:eqtype) (#v:Type0) (hashf:(k -> SZ.t)) (l:pos_us)
-//   requires emp
-//   returns ht:ht_t k v
-//   ensures exists* pht. models ht pht ** pure (pht == mk_init_pht hashf l)
-// {
-//   let contents = V.alloc #(cell k v) Clean l;
-//   let ht = mk_ht l hashf contents;
-//   let pht = Ghost.hide (mk_init_pht #k #v hashf l);
-//   rewrite (V.pts_to contents (Seq.create (SZ.v l) Clean))
-//        as (V.pts_to ht.contents pht.repr.seq);
-//   fold models;
-//   admit ()
-// }
-// ```
+```pulse
+fn dealloc (#k:eqtype) (#v:Type0) (ht:ht_t k v)
+  requires exists* pht. models ht pht
+  ensures emp
+{
+  open SZ;
+  with pht. assert (models ht pht);
+  unfold models;
+  V.free ht.contents;
+}
+```
 
-// ```pulse
-// fn dealloc (#k:eqtype) (#v:Type0) (ht:ht_t k v)
-//   requires exists* pht. models ht pht
-//   ensures emp
-// {
-//   open SZ;
-//   with pht. assert (models ht pht);
-//   unfold models;
-//   V.free ht.contents;
-// }
-// ```
-
-// let sz_add (x y : SZ.t)
-//   : o:option SZ.t { Some? o ==> SZ.v (Some?.v o) == SZ.v x + SZ.v y } 
-//   = let open SZ in
-//     if x <=^ 0xffffsz
-//     then (
-//       if (y <=^ 0xffffsz -^ x)
-//       then Some (x +^ y)
-//       else None
-//     )
-//     else None
+let sz_add (x y : SZ.t)
+  : o:option SZ.t { Some? o ==> SZ.v (Some?.v o) == SZ.v x + SZ.v y } 
+  = let open SZ in
+    if x <=^ 0xffffsz
+    then (
+      if (y <=^ 0xffffsz -^ x)
+      then Some (x +^ y)
+      else None
+    )
+    else None
 
 
-// let size_t_mod (x:SZ.t) (y : SZ.t { y =!= 0sz }) 
-// : z:SZ.t { SZ.v z == SZ.v x % SZ.v y }
-//   = SZ.(x %^ y)
+let size_t_mod (x:SZ.t) (y : SZ.t { y =!= 0sz }) 
+: z:SZ.t { SZ.v z == SZ.v x % SZ.v y }
+  = SZ.(x %^ y)
 
-// #push-options "--z3rlimit_factor 4 --query_stats"
-// ```pulse
-// fn pulse_lookup_index (#kt:eqtype) (#vt:Type0)
-//   (#ht:erased (ht_t kt vt))
-//   (#pht:erased (pht_t kt vt))
-//   (r:erased (ref (ht_t kt vt)))
-//   (r_sz:ref pos_us)
-//   (r_hashf:ref (kt -> SZ.t))
-//   (r_contents:ref (V.vec (cell kt vt)))
-//   // (res:(ref pos_us & ref (kt -> SZ.t) & ref (V.vec (cell kt vt))))
-//   (k:kt)
-//   requires exploded_vp r ht r_sz r_hashf r_contents ** models ht pht
-//   returns  p:bool & option (vt & SZ.t)
-//   ensures  exploded_vp r ht r_sz r_hashf r_contents ** models ht pht ** 
-//            pure ( fst p ==> (snd p) == PHT.lookup_index_us pht k )
-// {
-//   open SZ;
+#push-options "--z3rlimit_factor 4 --query_stats"
+```pulse
+fn pulse_lookup_index (#kt:eqtype) (#vt:Type0)
+  (#ht:erased (ht_t kt vt))
+  (#pht:erased (pht_t kt vt))
+  (r:erased (ref (ht_t kt vt)))
+  (r_sz:ref pos_us)
+  (r_hashf:ref (kt -> SZ.t))
+  (r_contents:ref (V.vec (cell kt vt)))
+  // (res:(ref pos_us & ref (kt -> SZ.t) & ref (V.vec (cell kt vt))))
+  (k:kt)
+  requires exploded_vp r ht r_sz r_hashf r_contents ** models ht pht
+  returns  p:bool & option (vt & SZ.t)
+  ensures  exploded_vp r ht r_sz r_hashf r_contents ** models ht pht ** 
+           pure ( fst p ==> (snd p) == PHT.lookup_index_us pht k )
+{
+  open SZ;
 
-//   unfold exploded_vp;
-//   let sz = !r_sz;
-//   let hash = ref_apply r_hashf k;
-//   fold (exploded_vp r ht r_sz r_hashf r_contents);
+  unfold exploded_vp;
+  let sz = !r_sz;
+  let hash = ref_apply r_hashf k;
+  fold (exploded_vp r ht r_sz r_hashf r_contents);
 
-//   let cidx = size_t_mod hash sz;
-//   let mut off = 0sz;
-//   let mut cont = true;
-//   let mut err = false;
-//   let mut ret = None #(vt & SZ.t);
-//   unfold models;
+  let cidx = size_t_mod hash sz;
+  let mut off = 0sz;
+  let mut cont = true;
+  let mut err = false;
+  let mut ret = None #(vt & SZ.t);
+  unfold models;
 
-//   while (let voff = !off;
-//          let vcont = !cont;
-//          let verr = !err; 
-//          (voff <=^ sz && vcont = true && verr = false)) 
-//   invariant b. exists* (voff:SZ.t) (vcont verr:bool). (
-//     exploded_vp r ht r_sz r_hashf r_contents **
-//     V.pts_to ht.contents pht.repr.seq **
-//     R.pts_to off voff **
-//     R.pts_to cont vcont **
-//     R.pts_to err verr **
-//     R.pts_to ret (if (vcont || verr) then None else (PHT.lookup_index_us pht k)) **
-//     pure (
-//       SZ.v ht.sz == pht_sz pht /\
-//       voff <=^ ht.sz /\
-//       walk_get_idx pht.repr (SZ.v cidx) k (SZ.v voff) 
-//         == lookup_repr_index pht.repr k /\
-//       b == (voff <=^ ht.sz && vcont = true && verr = false)
-//     ))
-//   {
-//     unfold exploded_vp;
-//     let voff = !off;
-//     if (voff = sz)
-//     {
-//       cont := false;
-//       assert (R.pts_to ret None);
-//       fold (exploded_vp r ht r_sz r_hashf r_contents);
-//     }
-//     else
-//     {
-//       let opt_sum = cidx `sz_add` voff;
-//       match opt_sum
-//       {
-//         Some sum -> 
-//         {
-//           let idx = size_t_mod sum sz;
-//           rewrite (V.pts_to ht.contents pht.repr.seq)
-//                as (V.pts_to (reveal (hide ht.contents)) (reveal (hide pht.repr.seq)));
-//           let c = V.vec_ref_read r_contents idx;
-//           rewrite (V.pts_to (reveal (hide ht.contents)) (reveal (hide pht.repr.seq)))
-//                as (V.pts_to ht.contents pht.repr.seq);
-//           match c
-//           {
-//             Used k' v' ->
-//             {
-//               if (k' = k)
-//               {
-//                 cont := false;
-//                 ret := Some (v', idx);
-//                 assert (pure (pht.repr @@ SZ.v idx == Used k' v'));
-//                 assert (pure (lookup_repr_index pht.repr k == Some (v', SZ.v idx)));
-//                 fold (exploded_vp r ht r_sz r_hashf r_contents);
-//               } else
-//               {
-//                 off := voff +^ 1sz;
-//                 assert (pure (walk_get_idx pht.repr (SZ.v cidx) k (SZ.v voff) 
-//                   == walk_get_idx pht.repr (SZ.v cidx) k (SZ.v (voff+^1sz))));
-//                 fold (exploded_vp r ht r_sz r_hashf r_contents);
-//               }
-//             }
-//             Clean ->
-//             {
-//               cont := false;
-//               assert (pure (walk_get_idx pht.repr (SZ.v cidx) k (SZ.v voff) == None));
-//               assert (R.pts_to ret (PHT.lookup_index_us pht k));
-//               fold (exploded_vp r ht r_sz r_hashf r_contents);
-//             }
-//             Zombie ->
-//             {
-//               off := voff +^ 1sz;
-//               assert (pure (walk_get_idx pht.repr (SZ.v cidx) k (SZ.v voff) 
-//                 == walk_get_idx pht.repr (SZ.v cidx) k (SZ.v (voff+^1sz))));
-//               fold (exploded_vp r ht r_sz r_hashf r_contents);
-//             }
-//           }
-//         }
-//         None ->
-//         { 
-//           // ERROR - add failed
-//           err := true;
-//           fold (exploded_vp r ht r_sz r_hashf r_contents);
-//         }
-//       }
-//     }
-//   };
-//   let verr = !err;
-//   let o = !ret;
-//   fold (models ht pht);
-//   if verr
-//   {
-//     (false,o)
-//   }
-//   else
-//   {
-//     assert (R.pts_to ret (PHT.lookup_index_us pht k));
-//     (true,o)
-//   }
-// }
-// ```
-// #pop-options
+  while (let voff = !off;
+         let vcont = !cont;
+         let verr = !err; 
+         (voff <=^ sz && vcont = true && verr = false)) 
+  invariant b. exists* (voff:SZ.t) (vcont verr:bool). (
+    exploded_vp r ht r_sz r_hashf r_contents **
+    V.pts_to ht.contents pht.repr.seq **
+    R.pts_to off voff **
+    R.pts_to cont vcont **
+    R.pts_to err verr **
+    R.pts_to ret (if (vcont || verr) then None else (PHT.lookup_index_us pht k)) **
+    pure (
+      SZ.v ht.sz == pht_sz pht /\
+      voff <=^ ht.sz /\
+      walk_get_idx pht.repr (SZ.v cidx) k (SZ.v voff) 
+        == lookup_repr_index pht.repr k /\
+      b == (voff <=^ ht.sz && vcont = true && verr = false)
+    ))
+  {
+    unfold exploded_vp;
+    let voff = !off;
+    if (voff = sz)
+    {
+      cont := false;
+      assert (R.pts_to ret None);
+      fold (exploded_vp r ht r_sz r_hashf r_contents);
+    }
+    else
+    {
+      let opt_sum = cidx `sz_add` voff;
+      match opt_sum
+      {
+        Some sum -> 
+        {
+          let idx = size_t_mod sum sz;
+          rewrite (V.pts_to ht.contents pht.repr.seq)
+               as (V.pts_to (reveal (hide ht.contents)) (reveal (hide pht.repr.seq)));
+          let c = V.vec_ref_read r_contents idx;
+          rewrite (V.pts_to (reveal (hide ht.contents)) (reveal (hide pht.repr.seq)))
+               as (V.pts_to ht.contents pht.repr.seq);
+          match c
+          {
+            Used k' v' ->
+            {
+              if (k' = k)
+              {
+                cont := false;
+                ret := Some (v', idx);
+                assert (pure (pht.repr @@ SZ.v idx == Used k' v'));
+                assert (pure (lookup_repr_index pht.repr k == Some (v', SZ.v idx)));
+                fold (exploded_vp r ht r_sz r_hashf r_contents);
+              } else
+              {
+                off := voff +^ 1sz;
+                assert (pure (walk_get_idx pht.repr (SZ.v cidx) k (SZ.v voff) 
+                  == walk_get_idx pht.repr (SZ.v cidx) k (SZ.v (voff+^1sz))));
+                fold (exploded_vp r ht r_sz r_hashf r_contents);
+              }
+            }
+            Clean ->
+            {
+              cont := false;
+              assert (pure (walk_get_idx pht.repr (SZ.v cidx) k (SZ.v voff) == None));
+              assert (R.pts_to ret (PHT.lookup_index_us pht k));
+              fold (exploded_vp r ht r_sz r_hashf r_contents);
+            }
+            Zombie ->
+            {
+              off := voff +^ 1sz;
+              assert (pure (walk_get_idx pht.repr (SZ.v cidx) k (SZ.v voff) 
+                == walk_get_idx pht.repr (SZ.v cidx) k (SZ.v (voff+^1sz))));
+              fold (exploded_vp r ht r_sz r_hashf r_contents);
+            }
+          }
+        }
+        None ->
+        { 
+          // ERROR - add failed
+          err := true;
+          fold (exploded_vp r ht r_sz r_hashf r_contents);
+        }
+      }
+    }
+  };
+  let verr = !err;
+  let o = !ret;
+  fold (models ht pht);
+  if verr
+  {
+    (false,o)
+  }
+  else
+  {
+    assert (R.pts_to ret (PHT.lookup_index_us pht k));
+    (true,o)
+  }
+}
+```
+#pop-options
 
-// ```pulse
-// fn lookup (#kt:eqtype) (#vt:Type0)
-//   (r:ref (ht_t kt vt)) (k:kt)
-//   (#ht:erased (ht_t kt vt))
-//   (#pht:erased (pht_t kt vt))
-//   requires pts_to r ht ** models ht pht
-//   returns  p:bool & option vt
-//   ensures  pts_to r ht ** models ht pht ** 
-//            pure ( fst p ==> (snd p) == PHT.lookup pht k )
-// {
-//   let res = explode_ref_ht_t r;
-//   match res
-//   {
-//     Mktuple3 r_sz r_hashf r_contents -> {
-//       rewrite (exploded_vp r ht (tfst res) (tsnd res) (tthd res))
-//            as (exploded_vp r ht r_sz r_hashf r_contents);
-//       rewrite (exploded_vp r ht r_sz r_hashf r_contents)
-//            as (exploded_vp (reveal (hide r)) ht r_sz r_hashf r_contents);
-//       let p = pulse_lookup_index (hide r) r_sz r_hashf r_contents k;
-//       rewrite (exploded_vp (reveal (hide r)) ht r_sz r_hashf r_contents)
-//            as (exploded_vp r ht r_sz r_hashf r_contents);
-//       unexplode_ref r r_sz r_hashf r_contents;
-//       if (fst p)
-//       {
-//         match (snd p)
-//         {
-//           Some p -> { (true, Some (fst p)) }
-//           None -> { (true, None #vt) }
-//         }
-//       } 
-//       else
-//       {
-//         (false, None #vt)
-//       }
-//     }
-//   }
-// }
-// ```
+```pulse
+fn lookup (#kt:eqtype) (#vt:Type0)
+  (r:ref (ht_t kt vt)) (k:kt)
+  (#ht:erased (ht_t kt vt))
+  (#pht:erased (pht_t kt vt))
+  requires pts_to r ht ** models ht pht
+  returns  p:bool & option vt
+  ensures  pts_to r ht ** models ht pht ** 
+           pure ( fst p ==> (snd p) == PHT.lookup pht k )
+{
+  let res = explode_ref_ht_t r;
+  match res
+  {
+    Mktuple3 r_sz r_hashf r_contents -> {
+      rewrite (exploded_vp r ht (tfst res) (tsnd res) (tthd res))
+           as (exploded_vp r ht r_sz r_hashf r_contents);
+      rewrite (exploded_vp r ht r_sz r_hashf r_contents)
+           as (exploded_vp (reveal (hide r)) ht r_sz r_hashf r_contents);
+      let p = pulse_lookup_index (hide r) r_sz r_hashf r_contents k;
+      rewrite (exploded_vp (reveal (hide r)) ht r_sz r_hashf r_contents)
+           as (exploded_vp r ht r_sz r_hashf r_contents);
+      unexplode_ref r r_sz r_hashf r_contents;
+      if (fst p)
+      {
+        match (snd p)
+        {
+          Some p -> { (true, Some (fst p)) }
+          None -> { (true, None #vt) }
+        }
+      } 
+      else
+      {
+        (false, None #vt)
+      }
+    }
+  }
+}
+```
 
-// ```pulse
-// fn insert (#kt:eqtype) (#vt:Type0)
-//   (r:ref (ht_t kt vt)) (k:kt) (v:vt)
-//   (#ht:erased (ht_t kt vt))
-//   (#pht:(p:erased (pht_t kt vt) { PHT.not_full p.repr }))
+```pulse
+fn insert (#kt:eqtype) (#vt:Type0)
+  (r:ref (ht_t kt vt)) (k:kt) (v:vt)
+  (#ht:erased (ht_t kt vt))
+  (#pht:(p:erased (pht_t kt vt) { PHT.not_full p.repr }))
   
-//   requires pts_to r ht ** models ht pht
-//   returns b:bool
-//   ensures exists* pht'.
-//     pts_to r ht ** models ht pht' **
-//     pure (if b
-//           then pht'== PHT.insert pht k v
-//           else pht'== pht)
-// {
-//   let res = explode_ref_ht_t r;
+  requires pts_to r ht ** models ht pht
+  returns b:bool
+  ensures exists* pht'.
+    pts_to r ht ** models ht pht' **
+    pure (if b
+          then pht'== PHT.insert pht k v
+          else pht'== pht)
+{
+  let res = explode_ref_ht_t r;
 
-//   match res {
+  match res {
 
-//   Mktuple3 r_sz r_hashf r_contents -> {
-//     rewrite (exploded_vp r ht (tfst res) (tsnd res) (tthd res))
-//          as (exploded_vp r ht r_sz r_hashf r_contents);
+  Mktuple3 r_sz r_hashf r_contents -> {
+    rewrite (exploded_vp r ht (tfst res) (tsnd res) (tthd res))
+         as (exploded_vp r ht r_sz r_hashf r_contents);
 
-//     unfold exploded_vp;
-//     let sz = !r_sz;
-//     let hash = ref_apply r_hashf k;
-//     fold (exploded_vp r ht r_sz r_hashf r_contents);
+    unfold exploded_vp;
+    let sz = !r_sz;
+    let hash = ref_apply r_hashf k;
+    fold (exploded_vp r ht r_sz r_hashf r_contents);
 
-//     let cidx = size_t_mod hash sz;
-//     let mut off = 0sz;
-//     let mut cont = true;
-//     let mut err = false;
+    let cidx = size_t_mod hash sz;
+    let mut off = 0sz;
+    let mut cont = true;
+    let mut err = false;
 
-//     unfold models;
-//     while
-//     (
-//       let vcont = !cont;
-//       let verr = !err;
-//       (vcont = true && verr = false)
-//     ) 
-//     invariant b. exists* (voff:SZ.t) (vcont verr:bool). (
-//       exploded_vp r ht r_sz r_hashf r_contents **
-//       R.pts_to off voff **
-//       R.pts_to cont vcont **
-//       R.pts_to err verr **
-//       V.pts_to ht.contents (if (vcont || verr) then pht.repr.seq else (PHT.insert pht k v).repr.seq) **
-//       pure (
-//         related ht pht /\
-//         SZ.(voff <=^ ht.sz) /\
-//         strong_all_used_not_by pht.repr (SZ.v cidx) (SZ.v voff) k /\
-//         walk pht.repr (SZ.v cidx) k (SZ.v voff) == lookup_repr pht.repr k /\
-//         insert_repr_walk #kt #vt #(pht_sz pht) #pht.spec pht.repr k v (SZ.v voff) (SZ.v cidx) () () 
-//           == insert_repr #kt #vt #(pht_sz pht) #pht.spec pht.repr k v /\
-//         b == (vcont = true && verr = false)
-//       ))
-//     {
-//       unfold exploded_vp;
-//       let voff = !off;
-//       if (voff = sz)
-//       {
-//         cont := false;
-//         full_not_full pht.repr k;
-//         assert (V.pts_to ht.contents pht.repr.seq);
-//         fold (exploded_vp r ht r_sz r_hashf r_contents);
-//       }
-//       else
-//       {
-//         let opt_sum = cidx `sz_add` voff;
-//         match opt_sum
-//         {
-//           Some sum ->
-//           {
-//             let idx = size_t_mod sum sz;
-//             rewrite (V.pts_to ht.contents pht.repr.seq)
-//                  as (V.pts_to (reveal (hide ht.contents)) (reveal (hide pht.repr.seq)));
-//             let c = V.vec_ref_read r_contents idx;
-//             rewrite (V.pts_to (reveal (hide ht.contents)) (reveal (hide pht.repr.seq)))
-//                  as (V.pts_to ht.contents pht.repr.seq);
+    unfold models;
+    while
+    (
+      let vcont = !cont;
+      let verr = !err;
+      (vcont = true && verr = false)
+    ) 
+    invariant b. exists* (voff:SZ.t) (vcont verr:bool). (
+      exploded_vp r ht r_sz r_hashf r_contents **
+      R.pts_to off voff **
+      R.pts_to cont vcont **
+      R.pts_to err verr **
+      V.pts_to ht.contents (if (vcont || verr) then pht.repr.seq else (PHT.insert pht k v).repr.seq) **
+      pure (
+        related ht pht /\
+        SZ.(voff <=^ ht.sz) /\
+        strong_all_used_not_by pht.repr (SZ.v cidx) (SZ.v voff) k /\
+        walk pht.repr (SZ.v cidx) k (SZ.v voff) == lookup_repr pht.repr k /\
+        insert_repr_walk #kt #vt #(pht_sz pht) #pht.spec pht.repr k v (SZ.v voff) (SZ.v cidx) () () 
+          == insert_repr #kt #vt #(pht_sz pht) #pht.spec pht.repr k v /\
+        b == (vcont = true && verr = false)
+      ))
+    {
+      unfold exploded_vp;
+      let voff = !off;
+      if (voff = sz)
+      {
+        cont := false;
+        full_not_full pht.repr k;
+        assert (V.pts_to ht.contents pht.repr.seq);
+        fold (exploded_vp r ht r_sz r_hashf r_contents);
+      }
+      else
+      {
+        let opt_sum = cidx `sz_add` voff;
+        match opt_sum
+        {
+          Some sum ->
+          {
+            let idx = size_t_mod sum sz;
+            rewrite (V.pts_to ht.contents pht.repr.seq)
+                 as (V.pts_to (reveal (hide ht.contents)) (reveal (hide pht.repr.seq)));
+            let c = V.vec_ref_read r_contents idx;
+            rewrite (V.pts_to (reveal (hide ht.contents)) (reveal (hide pht.repr.seq)))
+                 as (V.pts_to ht.contents pht.repr.seq);
 
-//             match c
-//             {
-//               Used k' v' -> { 
-//                 if (k' = k) {
-//                   assert (V.pts_to ht.contents pht.repr.seq);
-//                   assert (pure ( SZ.v idx < Seq.length pht.repr.seq));
-//                   rewrite (V.pts_to ht.contents pht.repr.seq)
-//                        as (V.pts_to (reveal (hide ht.contents)) (reveal (hide pht.repr.seq)));
-//                   V.vec_ref_write r_contents idx (mk_used_cell k v);
-//                   assert (pure ((insert_repr #kt #vt #(pht_sz pht) #pht.spec pht.repr k v).seq `Seq.equal` 
-//                                 Seq.upd pht.repr.seq (SZ.v idx) (mk_used_cell k v)));
-//                   rewrite (V.pts_to (reveal (hide ht.contents)) (Seq.upd (reveal (hide pht.repr.seq)) (SZ.v idx) (mk_used_cell k v)))
-//                        as (V.pts_to ht.contents (insert_repr #kt #vt #(pht_sz pht) #pht.spec pht.repr k v).seq);
-//                   cont := false;
-//                   fold (exploded_vp r ht r_sz r_hashf r_contents);
-//                 } else {
-//                   off := SZ.(voff +^ 1sz);
-//                   fold (exploded_vp r ht r_sz r_hashf r_contents);
-//                 } 
-//               }
-//               Clean -> {
-//                 rewrite (V.pts_to ht.contents pht.repr.seq)
-//                      as (V.pts_to (reveal (hide ht.contents)) (reveal (hide pht.repr.seq)));
-//                 V.vec_ref_write r_contents idx (mk_used_cell k v);
-//                 assert (pure ((insert_repr #kt #vt #(pht_sz pht) #pht.spec pht.repr k v).seq `Seq.equal` 
-//                               Seq.upd pht.repr.seq (SZ.v idx) (mk_used_cell k v)));
-//                 rewrite (V.pts_to (reveal (hide ht.contents)) (Seq.upd (reveal (hide pht.repr.seq)) (SZ.v idx) (mk_used_cell k v)))
-//                      as (V.pts_to ht.contents (insert_repr #kt #vt #(pht_sz pht) #pht.spec pht.repr k v).seq);
-//                 cont := false;
-//                 fold (exploded_vp r ht r_sz r_hashf r_contents);
-//               }
-//               Zombie ->
-//               {
-//                 fold (models ht pht);
-//                 fold (exploded_vp r ht r_sz r_hashf r_contents);
-//                 rewrite (exploded_vp r ht r_sz r_hashf r_contents)
-//                      as (exploded_vp (reveal (hide r)) ht r_sz r_hashf r_contents);
-//                 let lookup_res = pulse_lookup_index (hide r) r_sz r_hashf r_contents k;
-//                 rewrite (exploded_vp (reveal (hide r)) ht r_sz r_hashf r_contents)
-//                      as (exploded_vp r ht r_sz r_hashf r_contents);
-//                 unfold models;
-//                 unfold exploded_vp;
+            match c
+            {
+              Used k' v' -> { 
+                if (k' = k) {
+                  assert (V.pts_to ht.contents pht.repr.seq);
+                  assert (pure ( SZ.v idx < Seq.length pht.repr.seq));
+                  rewrite (V.pts_to ht.contents pht.repr.seq)
+                       as (V.pts_to (reveal (hide ht.contents)) (reveal (hide pht.repr.seq)));
+                  V.vec_ref_write r_contents idx (mk_used_cell k v);
+                  assert (pure ((insert_repr #kt #vt #(pht_sz pht) #pht.spec pht.repr k v).seq `Seq.equal` 
+                                Seq.upd pht.repr.seq (SZ.v idx) (mk_used_cell k v)));
+                  rewrite (V.pts_to (reveal (hide ht.contents)) (Seq.upd (reveal (hide pht.repr.seq)) (SZ.v idx) (mk_used_cell k v)))
+                       as (V.pts_to ht.contents (insert_repr #kt #vt #(pht_sz pht) #pht.spec pht.repr k v).seq);
+                  cont := false;
+                  fold (exploded_vp r ht r_sz r_hashf r_contents);
+                } else {
+                  off := SZ.(voff +^ 1sz);
+                  fold (exploded_vp r ht r_sz r_hashf r_contents);
+                } 
+              }
+              Clean -> {
+                rewrite (V.pts_to ht.contents pht.repr.seq)
+                     as (V.pts_to (reveal (hide ht.contents)) (reveal (hide pht.repr.seq)));
+                V.vec_ref_write r_contents idx (mk_used_cell k v);
+                assert (pure ((insert_repr #kt #vt #(pht_sz pht) #pht.spec pht.repr k v).seq `Seq.equal` 
+                              Seq.upd pht.repr.seq (SZ.v idx) (mk_used_cell k v)));
+                rewrite (V.pts_to (reveal (hide ht.contents)) (Seq.upd (reveal (hide pht.repr.seq)) (SZ.v idx) (mk_used_cell k v)))
+                     as (V.pts_to ht.contents (insert_repr #kt #vt #(pht_sz pht) #pht.spec pht.repr k v).seq);
+                cont := false;
+                fold (exploded_vp r ht r_sz r_hashf r_contents);
+              }
+              Zombie ->
+              {
+                fold (models ht pht);
+                fold (exploded_vp r ht r_sz r_hashf r_contents);
+                rewrite (exploded_vp r ht r_sz r_hashf r_contents)
+                     as (exploded_vp (reveal (hide r)) ht r_sz r_hashf r_contents);
+                let lookup_res = pulse_lookup_index (hide r) r_sz r_hashf r_contents k;
+                rewrite (exploded_vp (reveal (hide r)) ht r_sz r_hashf r_contents)
+                     as (exploded_vp r ht r_sz r_hashf r_contents);
+                unfold models;
+                unfold exploded_vp;
 
-//                 if (fst lookup_res)
-//                 {
-//                   let o = snd lookup_res;
-//                   match o
-//                   {
-//                     Some p ->
-//                     {
-//                       rewrite (V.pts_to ht.contents pht.repr.seq)
-//                            as (V.pts_to (reveal (hide ht.contents)) (reveal (hide pht.repr.seq)));
-//                       V.vec_ref_write r_contents (snd p) Zombie;
-//                       V.vec_ref_write r_contents idx (mk_used_cell k v);
-//                       cont := false;
-//                       assert (pure ((insert_repr #kt #vt #(pht_sz pht) #pht.spec pht.repr k v).seq `Seq.equal` 
-//                                     Seq.upd (Seq.upd pht.repr.seq (SZ.v (snd p)) Zombie) (SZ.v idx) (mk_used_cell k v)));
-//                       rewrite (V.pts_to (reveal (hide ht.contents))
-//                                         (Seq.upd (Seq.upd (reveal (hide pht.repr.seq)) (SZ.v (snd p)) Zombie) (SZ.v idx) (mk_used_cell k v)))
-//                            as (V.pts_to ht.contents (insert_repr #kt #vt #(pht_sz pht) #pht.spec pht.repr k v).seq);
-//                       fold (exploded_vp r ht r_sz r_hashf r_contents);
-//                     }
-//                     None ->
-//                     {
-//                       rewrite (V.pts_to ht.contents pht.repr.seq)
-//                            as (V.pts_to (reveal (hide ht.contents)) (reveal (hide pht.repr.seq)));
-//                       V.vec_ref_write r_contents idx (mk_used_cell k v);                    
-//                       cont := false;
-//                       assert (pure ((insert_repr #kt #vt #(pht_sz pht) #pht.spec pht.repr k v).seq `Seq.equal`
-//                                     Seq.upd pht.repr.seq (SZ.v idx) (mk_used_cell k v)));
-//                       rewrite (V.pts_to (reveal (hide ht.contents)) (Seq.upd (reveal (hide pht.repr.seq)) (SZ.v idx) (mk_used_cell k v)))
-//                            as (V.pts_to ht.contents (insert_repr #kt #vt #(pht_sz pht) #pht.spec pht.repr k v).seq);
-//                       fold (exploded_vp r ht r_sz r_hashf r_contents);
-//                     }
-//                   }
-//                 }
-//                 else
-//                 {
-//                   // ERROR - lookup failed
-//                   err := true;
-//                   fold (exploded_vp r ht r_sz r_hashf r_contents);
-//                 }
-//               }
-//             }
-//           }
-//           None ->
-//           {
-//             // ERROR - add failed
-//             err := true;
-//             fold (exploded_vp r ht r_sz r_hashf r_contents);
-//           }
-//         }
-//       }
-//     };
-//     unexplode_ref r r_sz r_hashf r_contents;
-//     let verr = !err;
-//     if verr
-//     {
-//       fold (models ht pht);
-//       false
-//     } else {
-//       assert (V.pts_to ht.contents (PHT.insert pht k v).repr.seq);
-//       fold (models ht (PHT.insert pht k v));
-//       true
-//     }
-//     }
-//   }
-// }
-// ```
+                if (fst lookup_res)
+                {
+                  let o = snd lookup_res;
+                  match o
+                  {
+                    Some p ->
+                    {
+                      rewrite (V.pts_to ht.contents pht.repr.seq)
+                           as (V.pts_to (reveal (hide ht.contents)) (reveal (hide pht.repr.seq)));
+                      V.vec_ref_write r_contents (snd p) Zombie;
+                      V.vec_ref_write r_contents idx (mk_used_cell k v);
+                      cont := false;
+                      assert (pure ((insert_repr #kt #vt #(pht_sz pht) #pht.spec pht.repr k v).seq `Seq.equal` 
+                                    Seq.upd (Seq.upd pht.repr.seq (SZ.v (snd p)) Zombie) (SZ.v idx) (mk_used_cell k v)));
+                      rewrite (V.pts_to (reveal (hide ht.contents))
+                                        (Seq.upd (Seq.upd (reveal (hide pht.repr.seq)) (SZ.v (snd p)) Zombie) (SZ.v idx) (mk_used_cell k v)))
+                           as (V.pts_to ht.contents (insert_repr #kt #vt #(pht_sz pht) #pht.spec pht.repr k v).seq);
+                      fold (exploded_vp r ht r_sz r_hashf r_contents);
+                    }
+                    None ->
+                    {
+                      rewrite (V.pts_to ht.contents pht.repr.seq)
+                           as (V.pts_to (reveal (hide ht.contents)) (reveal (hide pht.repr.seq)));
+                      V.vec_ref_write r_contents idx (mk_used_cell k v);                    
+                      cont := false;
+                      assert (pure ((insert_repr #kt #vt #(pht_sz pht) #pht.spec pht.repr k v).seq `Seq.equal`
+                                    Seq.upd pht.repr.seq (SZ.v idx) (mk_used_cell k v)));
+                      rewrite (V.pts_to (reveal (hide ht.contents)) (Seq.upd (reveal (hide pht.repr.seq)) (SZ.v idx) (mk_used_cell k v)))
+                           as (V.pts_to ht.contents (insert_repr #kt #vt #(pht_sz pht) #pht.spec pht.repr k v).seq);
+                      fold (exploded_vp r ht r_sz r_hashf r_contents);
+                    }
+                  }
+                }
+                else
+                {
+                  // ERROR - lookup failed
+                  err := true;
+                  fold (exploded_vp r ht r_sz r_hashf r_contents);
+                }
+              }
+            }
+          }
+          None ->
+          {
+            // ERROR - add failed
+            err := true;
+            fold (exploded_vp r ht r_sz r_hashf r_contents);
+          }
+        }
+      }
+    };
+    unexplode_ref r r_sz r_hashf r_contents;
+    let verr = !err;
+    if verr
+    {
+      fold (models ht pht);
+      false
+    } else {
+      assert (V.pts_to ht.contents (PHT.insert pht k v).repr.seq);
+      fold (models ht (PHT.insert pht k v));
+      true
+    }
+    }
+  }
+}
+```
 
-// ```pulse
-// fn delete (#kt:eqtype) (#vt:Type0)
-//   (r:ref (ht_t kt vt)) (k:kt)
-//   (#ht:erased (ht_t kt vt))
-//   (#pht:erased (pht_t kt vt))
-//   requires pts_to r ht ** models ht pht
-//   returns b:bool
-//   ensures exists* pht'.
-//     pts_to r ht **
-//     models ht pht' **
-//     pure (if b then pht' == PHT.delete pht k else pht' == pht)
-// {
-//   let res = explode_ref_ht_t r;
+```pulse
+fn delete (#kt:eqtype) (#vt:Type0)
+  (r:ref (ht_t kt vt)) (k:kt)
+  (#ht:erased (ht_t kt vt))
+  (#pht:erased (pht_t kt vt))
+  requires pts_to r ht ** models ht pht
+  returns b:bool
+  ensures exists* pht'.
+    pts_to r ht **
+    models ht pht' **
+    pure (if b then pht' == PHT.delete pht k else pht' == pht)
+{
+  let res = explode_ref_ht_t r;
 
-//   match res {
+  match res {
 
-//   Mktuple3 r_sz r_hashf r_contents -> {
-//   rewrite (exploded_vp r ht (tfst res) (tsnd res) (tthd res))
-//        as (exploded_vp r ht r_sz r_hashf r_contents);
+  Mktuple3 r_sz r_hashf r_contents -> {
+  rewrite (exploded_vp r ht (tfst res) (tsnd res) (tthd res))
+       as (exploded_vp r ht r_sz r_hashf r_contents);
   
-//   unfold (exploded_vp r ht r_sz r_hashf r_contents);
-//   let sz = !r_sz;
-//   let hash = ref_apply r_hashf k;
-//   fold (exploded_vp r ht r_sz r_hashf r_contents);
+  unfold (exploded_vp r ht r_sz r_hashf r_contents);
+  let sz = !r_sz;
+  let hash = ref_apply r_hashf k;
+  fold (exploded_vp r ht r_sz r_hashf r_contents);
 
-//   let cidx = size_t_mod hash sz;
-//   let mut off = 0sz;
-//   let mut cont = true;
-//   let mut err = false;
+  let cidx = size_t_mod hash sz;
+  let mut off = 0sz;
+  let mut cont = true;
+  let mut err = false;
 
-//   unfold (models ht pht);
-//   while 
-//   (
-//     let vcont = !cont;
-//     let verr = !err; 
-//     (vcont = true && verr = false)
-//   )
-//   invariant b. exists* (voff:SZ.t) (vcont verr:bool). (
-//     exploded_vp r ht r_sz r_hashf r_contents **
-//     R.pts_to off voff **
-//     R.pts_to cont vcont **
-//     R.pts_to err verr **
-//     V.pts_to ht.contents (if (vcont || verr) then pht.repr.seq else (PHT.delete pht k).repr.seq) **
-//     pure (
-//       SZ.v ht.sz == pht_sz pht /\
-//       SZ.(voff <=^ ht.sz) /\
-//       all_used_not_by pht.repr (SZ.v cidx) (SZ.v voff) k /\
-//       walk pht.repr (SZ.v cidx) k (SZ.v voff) == lookup_repr pht.repr k /\
-//       delete_repr_walk #kt #vt #(pht_sz pht) #pht.spec pht.repr k (SZ.v voff) (SZ.v cidx) () () 
-//         == delete_repr #kt #vt #(pht_sz pht) #pht.spec pht.repr k /\
-//       b == (vcont = true && verr = false)
-//     ))
-//   {
-//     unfold (exploded_vp r ht r_sz r_hashf r_contents);
-//     let voff = !off;
-//     if (voff = sz)
-//     {
-//       cont := false;
-//       assert (V.pts_to ht.contents pht.repr.seq);
-//       fold (exploded_vp r ht r_sz r_hashf r_contents);
-//     }
-//     else
-//     {
-//       let opt_sum = cidx `sz_add` voff;
-//       match opt_sum
-//       {
-//         Some sum ->
-//         {
-//           let idx = size_t_mod sum sz;
-//           rewrite (V.pts_to ht.contents pht.repr.seq)
-//                as (V.pts_to (reveal (hide ht.contents)) (reveal (hide pht.repr.seq)));
-//           let c = V.vec_ref_read r_contents idx;
-//           rewrite (V.pts_to (reveal (hide ht.contents)) (reveal (hide pht.repr.seq)))
-//                as (V.pts_to ht.contents pht.repr.seq);
+  unfold (models ht pht);
+  while 
+  (
+    let vcont = !cont;
+    let verr = !err; 
+    (vcont = true && verr = false)
+  )
+  invariant b. exists* (voff:SZ.t) (vcont verr:bool). (
+    exploded_vp r ht r_sz r_hashf r_contents **
+    R.pts_to off voff **
+    R.pts_to cont vcont **
+    R.pts_to err verr **
+    V.pts_to ht.contents (if (vcont || verr) then pht.repr.seq else (PHT.delete pht k).repr.seq) **
+    pure (
+      SZ.v ht.sz == pht_sz pht /\
+      SZ.(voff <=^ ht.sz) /\
+      all_used_not_by pht.repr (SZ.v cidx) (SZ.v voff) k /\
+      walk pht.repr (SZ.v cidx) k (SZ.v voff) == lookup_repr pht.repr k /\
+      delete_repr_walk #kt #vt #(pht_sz pht) #pht.spec pht.repr k (SZ.v voff) (SZ.v cidx) () () 
+        == delete_repr #kt #vt #(pht_sz pht) #pht.spec pht.repr k /\
+      b == (vcont = true && verr = false)
+    ))
+  {
+    unfold (exploded_vp r ht r_sz r_hashf r_contents);
+    let voff = !off;
+    if (voff = sz)
+    {
+      cont := false;
+      assert (V.pts_to ht.contents pht.repr.seq);
+      fold (exploded_vp r ht r_sz r_hashf r_contents);
+    }
+    else
+    {
+      let opt_sum = cidx `sz_add` voff;
+      match opt_sum
+      {
+        Some sum ->
+        {
+          let idx = size_t_mod sum sz;
+          rewrite (V.pts_to ht.contents pht.repr.seq)
+               as (V.pts_to (reveal (hide ht.contents)) (reveal (hide pht.repr.seq)));
+          let c = V.vec_ref_read r_contents idx;
+          rewrite (V.pts_to (reveal (hide ht.contents)) (reveal (hide pht.repr.seq)))
+               as (V.pts_to ht.contents pht.repr.seq);
 
-//           match c
-//           {
-//             Used k' v' ->
-//             { 
-//               if (k' = k)
-//               {
-//                 rewrite (V.pts_to ht.contents pht.repr.seq)
-//                      as (V.pts_to (reveal (hide ht.contents)) (reveal (hide pht.repr.seq)));
-//                 V.vec_ref_write r_contents idx Zombie;
-//                 cont := false;
-//                 assert (pure (pht.repr @@ SZ.v idx == Used k v'));
-//                 assert (pure (Seq.upd pht.repr.seq (SZ.v idx) Zombie  `Seq.equal`
-//                               (PHT.delete pht k).repr.seq));
-//                 rewrite (V.pts_to (reveal (hide ht.contents)) (Seq.upd (reveal (hide pht.repr.seq)) (SZ.v idx) Zombie))
-//                      as (V.pts_to ht.contents (PHT.delete pht k).repr.seq);
-//                 fold (exploded_vp r ht r_sz r_hashf r_contents);
-//               }
-//               else
-//               {
-//                 off := SZ.(voff +^ 1sz);
-//                 fold (exploded_vp r ht r_sz r_hashf r_contents);
-//               } 
-//             }
-//             Clean ->
-//             {
-//               cont := false;
-//               assert (pure (pht.repr == (PHT.delete pht k).repr));
-//               fold (exploded_vp r ht r_sz r_hashf r_contents);
-//             }
-//             Zombie ->
-//             {
-//               off := SZ.(voff +^ 1sz);
-//               fold (exploded_vp r ht r_sz r_hashf r_contents);
-//             }
-//           }
-//         }
-//         None ->
-//         {
-//           // ERROR - add failed
-//           err := false;
-//           fold (exploded_vp r ht r_sz r_hashf r_contents);
-//         }
-//       }
-//     }
-//   };
-//   unexplode_ref r r_sz r_hashf r_contents;
-//   let verr = !err;
-//   if verr
-//   {
-//     fold (models ht pht);
-//     false
-//   }
-//   else
-//   {
-//     fold (models ht (PHT.delete pht k));
-//     true
-//   }
-//   }
-//   }
-// }
-// ```
+          match c
+          {
+            Used k' v' ->
+            { 
+              if (k' = k)
+              {
+                rewrite (V.pts_to ht.contents pht.repr.seq)
+                     as (V.pts_to (reveal (hide ht.contents)) (reveal (hide pht.repr.seq)));
+                V.vec_ref_write r_contents idx Zombie;
+                cont := false;
+                assert (pure (pht.repr @@ SZ.v idx == Used k v'));
+                assert (pure (Seq.upd pht.repr.seq (SZ.v idx) Zombie  `Seq.equal`
+                              (PHT.delete pht k).repr.seq));
+                rewrite (V.pts_to (reveal (hide ht.contents)) (Seq.upd (reveal (hide pht.repr.seq)) (SZ.v idx) Zombie))
+                     as (V.pts_to ht.contents (PHT.delete pht k).repr.seq);
+                fold (exploded_vp r ht r_sz r_hashf r_contents);
+              }
+              else
+              {
+                off := SZ.(voff +^ 1sz);
+                fold (exploded_vp r ht r_sz r_hashf r_contents);
+              } 
+            }
+            Clean ->
+            {
+              cont := false;
+              assert (pure (pht.repr == (PHT.delete pht k).repr));
+              fold (exploded_vp r ht r_sz r_hashf r_contents);
+            }
+            Zombie ->
+            {
+              off := SZ.(voff +^ 1sz);
+              fold (exploded_vp r ht r_sz r_hashf r_contents);
+            }
+          }
+        }
+        None ->
+        {
+          // ERROR - add failed
+          err := false;
+          fold (exploded_vp r ht r_sz r_hashf r_contents);
+        }
+      }
+    }
+  };
+  unexplode_ref r r_sz r_hashf r_contents;
+  let verr = !err;
+  if verr
+  {
+    fold (models ht pht);
+    false
+  }
+  else
+  {
+    fold (models ht (PHT.delete pht k));
+    true
+  }
+  }
+  }
+}
+```
 
-// let is_used (#k:eqtype) (#v:Type0) (c:cell k v) : bool =
-//   match c with
-//   | Used _ _ -> true
-//   | _ -> false
+let is_used (#k:eqtype) (#v:Type0) (c:cell k v) : bool =
+  match c with
+  | Used _ _ -> true
+  | _ -> false
 
-// ```pulse
-// fn not_full (#kt:eqtype) (#vt:Type0)
-//   (r:ref (ht_t kt vt))
-//   (#ht:erased (ht_t kt vt))
-//   (#pht:erased (pht_t kt vt))
-//   requires pts_to r ht ** models ht pht
-//   returns b:bool
-//   ensures pts_to r ht ** models ht pht ** 
-//           pure (b ==> PHT.not_full pht.repr)
-// {
-//   let res = explode_ref_ht_t r;
+```pulse
+fn not_full (#kt:eqtype) (#vt:Type0)
+  (r:ref (ht_t kt vt))
+  (#ht:erased (ht_t kt vt))
+  (#pht:erased (pht_t kt vt))
+  requires pts_to r ht ** models ht pht
+  returns b:bool
+  ensures pts_to r ht ** models ht pht ** 
+          pure (b ==> PHT.not_full pht.repr)
+{
+  let res = explode_ref_ht_t r;
 
-//   match res {
+  match res {
  
-//   Mktuple3 r_sz r_hashf r_contents -> {
+  Mktuple3 r_sz r_hashf r_contents -> {
 
-//   rewrite (exploded_vp r ht (tfst res) (tsnd res) (tthd res))
-//        as (exploded_vp r ht r_sz r_hashf r_contents);
+  rewrite (exploded_vp r ht (tfst res) (tsnd res) (tthd res))
+       as (exploded_vp r ht r_sz r_hashf r_contents);
 
-//   let mut i = 0sz;
-//   unfold (models ht pht);
+  let mut i = 0sz;
+  unfold (models ht pht);
 
-//   unfold (exploded_vp r ht r_sz r_hashf r_contents);
-//   let sz = !r_sz;
-//   fold (exploded_vp r ht r_sz r_hashf r_contents);
+  unfold (exploded_vp r ht r_sz r_hashf r_contents);
+  let sz = !r_sz;
+  fold (exploded_vp r ht r_sz r_hashf r_contents);
 
-//   while
-//   (
-//     let vi = !i;  
-//     if SZ.(vi <^ sz)
-//     {
-//       unfold (exploded_vp r ht r_sz r_hashf r_contents);
-//       rewrite (V.pts_to ht.contents pht.repr.seq)
-//            as (V.pts_to (reveal (hide ht.contents)) (reveal (hide pht.repr.seq)));
-//       let c = V.vec_ref_read r_contents vi;
-//       rewrite (V.pts_to (reveal (hide ht.contents)) (reveal (hide pht.repr.seq)))
-//            as (V.pts_to ht.contents pht.repr.seq);
-//       fold (exploded_vp r ht r_sz r_hashf r_contents);
-//       is_used c
-//     }
-//     else 
-//     { 
-//       false
-//     }
-//   )
-//   invariant b. exists* (vi:SZ.t). (
-//     exploded_vp r ht r_sz r_hashf r_contents **
-//     V.pts_to ht.contents pht.repr.seq **
-//     R.pts_to i vi **
-//     pure (
-//       SZ.v ht.sz == pht_sz pht /\
-//       SZ.(vi <=^ ht.sz) /\
-//       (b == (SZ.(vi <^ ht.sz) && Used? (pht.repr @@ (SZ.v vi)))) /\
-//       (forall (i:nat). i < SZ.v vi ==> is_used (pht.repr @@ i))
-//     )
-//   )
-//   {
-//     let vi = !i;
-//     i := SZ.(vi +^ 1sz);
-//   };
-//   unexplode_ref r r_sz r_hashf r_contents;
-//   let vi = !i;
-//   let res = SZ.(vi <^ sz);
-//   fold (models ht pht);  
-//   res
-// }
-// }
-// }
-// ```
+  while
+  (
+    let vi = !i;  
+    if SZ.(vi <^ sz)
+    {
+      unfold (exploded_vp r ht r_sz r_hashf r_contents);
+      rewrite (V.pts_to ht.contents pht.repr.seq)
+           as (V.pts_to (reveal (hide ht.contents)) (reveal (hide pht.repr.seq)));
+      let c = V.vec_ref_read r_contents vi;
+      rewrite (V.pts_to (reveal (hide ht.contents)) (reveal (hide pht.repr.seq)))
+           as (V.pts_to ht.contents pht.repr.seq);
+      fold (exploded_vp r ht r_sz r_hashf r_contents);
+      is_used c
+    }
+    else 
+    { 
+      false
+    }
+  )
+  invariant b. exists* (vi:SZ.t). (
+    exploded_vp r ht r_sz r_hashf r_contents **
+    V.pts_to ht.contents pht.repr.seq **
+    R.pts_to i vi **
+    pure (
+      SZ.v ht.sz == pht_sz pht /\
+      SZ.(vi <=^ ht.sz) /\
+      (b == (SZ.(vi <^ ht.sz) && Used? (pht.repr @@ (SZ.v vi)))) /\
+      (forall (i:nat). i < SZ.v vi ==> is_used (pht.repr @@ i))
+    )
+  )
+  {
+    let vi = !i;
+    i := SZ.(vi +^ 1sz);
+  };
+  unexplode_ref r r_sz r_hashf r_contents;
+  let vi = !i;
+  let res = SZ.(vi <^ sz);
+  fold (models ht pht);  
+  res
+}
+}
+}
+```
 
-// let hash_us (k:SZ.t) : SZ.t = k
+let hash_us (k:SZ.t) : SZ.t = k
 
-// let init_not_full (#kt:eqtype) (#vt:eqtype) (hashf:kt -> SZ.t) (l:pos_us)
-//   : Lemma (Pulse.Lib.HashTable.Spec.not_full (mk_init_pht #kt #vt hashf l).repr)
-//   = assert (~(Used? ((mk_init_pht #kt #vt hashf l).repr @@ 0)))
+let init_not_full (#kt:eqtype) (#vt:eqtype) (hashf:kt -> SZ.t) (l:pos_us)
+  : Lemma (Pulse.Lib.HashTable.Spec.not_full (mk_init_pht #kt #vt hashf l).repr)
+  = assert (~(Used? ((mk_init_pht #kt #vt hashf l).repr @@ 0)))
 
-// ```pulse
-// fn test_mono ()
-//   requires emp
-//   ensures emp
-// {
-//    let htc = alloc #SZ.t #SZ.t hash_us 128sz;
-//    with pht. assert (models htc pht);
-//    let ht = R.alloc htc;
-//    init_not_full #SZ.t #SZ.t hash_us 128sz;
-//    rewrite (models htc pht) as (models (reveal (hide htc)) pht);
-//    let b = insert ht 0sz 17sz;
-//    if (b) {
-//      let v = lookup ht 0sz;
-//      if (fst v) {
-//        assert pure (snd v == Some 17sz);
-//        R.free ht;
-//        with pht. assert (models (reveal (hide htc)) pht);
-//        rewrite (models (reveal (hide htc)) pht) as (models htc pht);
-//        dealloc htc
-//      }
-//      else {
-//       R.free ht;
-//       with pht. assert (models (reveal (hide htc)) pht);
-//       rewrite (models (reveal (hide htc)) pht) as (models htc pht);
-//       dealloc htc
-//      }
-//    }
-//    else {
-//     let b = delete ht 0sz;
-//     let b' = not_full ht;
-//     R.free ht;
-//     with pht. assert (models (reveal (hide htc)) pht);
-//     rewrite (models (reveal (hide htc)) pht) as (models htc pht);
-//     dealloc htc
-//    } 
-// }
-// ```
+```pulse
+fn test_mono ()
+  requires emp
+  ensures emp
+{
+   let htc = alloc #SZ.t #SZ.t hash_us 128sz;
+   with pht. assert (models htc pht);
+   let ht = R.alloc htc;
+   init_not_full #SZ.t #SZ.t hash_us 128sz;
+   rewrite (models htc pht) as (models (reveal (hide htc)) pht);
+   let b = insert ht 0sz 17sz;
+   if (b) {
+     let v = lookup ht 0sz;
+     if (fst v) {
+       assert pure (snd v == Some 17sz);
+       R.free ht;
+       with pht. assert (models (reveal (hide htc)) pht);
+       rewrite (models (reveal (hide htc)) pht) as (models htc pht);
+       dealloc htc
+     }
+     else {
+      R.free ht;
+      with pht. assert (models (reveal (hide htc)) pht);
+      rewrite (models (reveal (hide htc)) pht) as (models htc pht);
+      dealloc htc
+     }
+   }
+   else {
+    let b = delete ht 0sz;
+    let b' = not_full ht;
+    R.free ht;
+    with pht. assert (models (reveal (hide htc)) pht);
+    rewrite (models (reveal (hide htc)) pht) as (models htc pht);
+    dealloc htc
+   } 
+}
+```
